Safe Deep Priority Conflicts

IPPGrammar.v
@@ -86,22 +86,61 @@ Inductive matches {g} : parse_tree g -> tree_pattern g -> Prop :=
 Definition matches_set {g} t (Q : tree_pattern g -> Prop) : Prop :=
   exists q, Q q /\ matches t q.
 
-Inductive conflict_free {g} (Q : tree_pattern g -> Prop) : parse_tree g -> Prop :=
+Inductive i_conflict_free {g} (Q : tree_pattern g -> Prop) : parse_tree g -> Prop :=
   | Atomic_cf l :
-      conflict_free Q (AtomicNode l)
+      i_conflict_free Q (AtomicNode l)
   | Infix_cf t1 o t2 :
       ~ matches_set (InfixNode t1 o t2) Q ->
-      conflict_free Q t1 ->
-      conflict_free Q t2 ->
-      conflict_free Q (InfixNode t1 o t2)
+      i_conflict_free Q t1 ->
+      i_conflict_free Q t2 ->
+      i_conflict_free Q (InfixNode t1 o t2)
   | Prefix_cf t o :
       ~ matches_set (PrefixNode o t) Q ->
-      conflict_free Q t ->
-      conflict_free Q (PrefixNode o t).
+      i_conflict_free Q t ->
+      i_conflict_free Q (PrefixNode o t).
   (* | PostfixNode_cf t o :
       ~ matches_set (PostfixNode t o) Q ->
       conflict_free Q t ->
       conflict_free Q (PostfixNode t o). *)
+
+Inductive matches_rm {g} : parse_tree g -> tree_pattern g -> Prop :=
+  | Match_rm t q :
+      matches t q ->
+      matches_rm t q
+  | InfixMatch_rm t1 o t2 q :
+      matches_rm t2 q ->
+      matches_rm (InfixNode t1 o t2) q
+  | PrefixMatch_rm o t q :
+      matches_rm t q ->
+      matches_rm (PrefixNode o t) q.
+
+Inductive matches_drm {g} : parse_tree g -> tree_pattern g -> Prop :=
+  | InfixMatch_drm t1 t2 q1 q2 o :
+      matches_rm t1 q1 ->
+      matches_rm t2 q2 ->
+      matches_drm (InfixNode t1 o t2) (InfixPatt q1 o q2)
+  | PrefixMatch_drm t q o : 
+      matches_rm t q ->
+      matches_drm (PrefixNode o t) (PrefixPatt o q).
+
+Definition matches_drm_set {g} t (Q : tree_pattern g -> Prop) : Prop :=
+  exists q, Q q /\ matches_drm t q.
+
+Inductive drm_conflict_free {g} (Q : tree_pattern g -> Prop) : parse_tree g -> Prop :=
+  | Atomic_drmcf l :
+      drm_conflict_free Q (AtomicNode l)
+  | Infix_drmcf t1 o t2 :
+      ~ matches_drm_set (InfixNode t1 o t2) Q ->
+      drm_conflict_free Q t1 ->
+      drm_conflict_free Q t2 ->
+      drm_conflict_free Q (InfixNode t1 o t2)
+  | Prefix_drmcf t o :
+      ~ matches_drm_set (PrefixNode o t) Q ->
+      drm_conflict_free Q t ->
+      drm_conflict_free Q (PrefixNode o t).
+
+Definition conflict_free {g} (Qi Qrm : tree_pattern g -> Prop) t :=
+  i_conflict_free Qi t /\ drm_conflict_free Qrm t.
 
 Record drules g := mkDrules {
   prio : prod g.(OP) -> prod g.(OP) -> Prop;
@@ -128,88 +167,31 @@ Definition CR_infix_infix {g} o1 o2 : tree_pattern g :=
 Definition CR_prefix_infix {g} o1 o2 : tree_pattern g :=
   PrefixPatt o1 (InfixPatt HPatt o2 HPatt).
 
-Inductive conflict_pattern {g} (pr : drules g) : tree_pattern g -> Prop :=
+Inductive i_conflict_pattern {g} (pr : drules g) : tree_pattern g -> Prop :=
   | CLeft o1 o2 : 
       pr.(left_a) (InfixProd o1) (InfixProd o2) ->
-      conflict_pattern pr (CR_infix_infix o1 o2)
+      i_conflict_pattern pr (CR_infix_infix o1 o2)
   | CRight o1 o2 : 
       pr.(right_a) (InfixProd o1) (InfixProd o2) ->
-      conflict_pattern pr (CL_infix_infix o1 o2)
+      i_conflict_pattern pr (CL_infix_infix o1 o2)
   | CPrio_infix_infix_1 o1 o2 :
       pr.(prio) (InfixProd o1) (InfixProd o2) ->
-      conflict_pattern pr (CL_infix_infix o1 o2)
+      i_conflict_pattern pr (CL_infix_infix o1 o2)
   | CPrio_infix_infix_2 o1 o2 :
       pr.(prio) (InfixProd o1) (InfixProd o2) ->
-      conflict_pattern pr (CR_infix_infix o1 o2)
-  | CPrio_infix_prefix o1 o2 :
-      pr.(prio) (InfixProd o1) (PrefixProd o2) ->
-      conflict_pattern pr (CL_infix_prefix o1 o2)
+      i_conflict_pattern pr (CR_infix_infix o1 o2)
   | CPrio_prefix_infix o1 o2 :
       pr.(prio) (PrefixProd o1) (InfixProd o2) ->
-      conflict_pattern pr (CR_prefix_infix o1 o2).
+      i_conflict_pattern pr (CR_prefix_infix o1 o2).
 
-Require Import MyUtils.
-
-Lemma dec_conflict_pattern {g} (pr : drules g) `{drules_dec pr} (q : tree_pattern g) :
-  Decision (conflict_pattern pr q).
-Proof.
-  destruct drules_dec0.
-  unfold Decision. destruct q.
-  - right. intro. inv H.
-  - destruct q1, q2.
-    + right. intro. inv H.
-    + destruct q2_1. destruct q2_2.
-      * replace (InfixPatt HPatt o (InfixPatt HPatt o0 HPatt)) with (CR_infix_infix o o0); try reflexivity.
-        specialize dec_prio0 with (p1 := InfixProd o) (p2 := InfixProd o0).
-        specialize dec_left_a0 with (p1 := InfixProd o) (p2 := InfixProd o0).
-        destruct dec_prio0, dec_left_a0; auto using CPrio_infix_infix_2, CLeft.
-        right. intro. inv H; contradiction.
-      * right. intro. inv H.
-      * right. intro. inv H.
-      * right. intro. inv H.
-      * right. intro. inv H.
-    + right. intro. inv H.
-    + destruct q1_1. destruct q1_2.
-      * replace (InfixPatt (InfixPatt HPatt o0 HPatt) o HPatt) with (CL_infix_infix o o0); try reflexivity.
-        specialize dec_prio0 with (p1 := InfixProd o) (p2 := InfixProd o0).
-        specialize dec_right_a0 with (p1 := InfixProd o) (p2 := InfixProd o0).
-        destruct dec_prio0, dec_right_a0; auto using CPrio_infix_infix_1, CRight.
-        right. intro. inv H; contradiction.
-      * right. intro. inv H.
-      * right. intro. inv H.
-      * right. intro. inv H.
-      * right. intro. inv H.
-    + right. intro. inv H.
-    + right. intro. inv H.
-    + destruct q1.
-      * replace (InfixPatt (PrefixPatt o0 HPatt) o HPatt) with (CL_infix_prefix o o0); try reflexivity.
-        specialize dec_prio0 with (p1 := InfixProd o) (p2 := PrefixProd o0).
-        destruct dec_prio0; auto using CPrio_infix_prefix.
-        right. intro. inv H; contradiction.
-      * right. intro. inv H.
-      * right. intro. inv H.
-    + right. intro. inv H.
-    + right. intro. inv H.
-  - destruct q.
-    + right. intro. inv H.
-    + destruct q1, q2.
-      * replace (PrefixPatt o (InfixPatt HPatt o0 HPatt)) with (CR_prefix_infix o o0); try reflexivity.
-        specialize dec_prio0 with (p1 := PrefixProd o) (p2 := InfixProd o0).
-        destruct dec_prio0; auto using CPrio_prefix_infix.
-        right. intro. inv H; contradiction.
-      * right. intro. inv H.
-      * right. intro. inv H.
-      * right. intro. inv H.
-      * right. intro. inv H.
-      * right. intro. inv H.
-      * right. intro. inv H.
-      * right. intro. inv H.
-      * right. intro. inv H.
-    + right. intro. inv H.
-Qed.
+Inductive rm_conflict_pattern {g} (pr : drules g) : tree_pattern g -> Prop :=
+  | CPrio_infix_prefix o1 o2 :
+      pr.(prio) (InfixProd o1) (PrefixProd o2) ->
+      rm_conflict_pattern pr (CL_infix_prefix o1 o2).
 
 Definition dlanguage {g} (pr : drules g) w : Prop :=
-  exists t, wf_parse_tree g t /\ yield t = w /\ conflict_free (conflict_pattern pr) t.
+  exists t, wf_parse_tree g t /\ yield t = w /\
+    conflict_free (i_conflict_pattern pr) (rm_conflict_pattern pr) t.
 
 Definition safe {g} (pr : drules g) : Prop :=
   forall w, language w -> dlanguage pr w.
@@ -220,37 +202,17 @@ Definition safe_pr {g} (pr : drules g) : Prop :=
     (pr.(prio) p2 p1 \/ (pr.(right_a)) p2 p1) ->
     False.
 
-Lemma safe_infix_infix {g} (pr : drules g) o1 o2 :
-  safe_pr pr ->
-  conflict_pattern pr (CL_infix_infix o1 o2) ->
-  conflict_pattern pr (CR_infix_infix o2 o1) ->
-  False.
-Proof.
-  intros H_safe H_CL H_CR. unfold safe_pr in H_safe.
-  inv H_CL; inv H_CR; eauto.
-Qed.
-
-Lemma safe_infix_prefix {g} (pr : drules g) o1 o2 :
-  safe_pr pr ->
-  conflict_pattern pr (CL_infix_prefix o1 o2) ->
-  conflict_pattern pr (CR_prefix_infix o2 o1) ->
-  False.
-Proof.
-  intros. unfold safe_pr in H.
-  inv H0; inv H1; eauto.
-Qed.
-
 Inductive linsert_one {g} (pr : drules g) (l1 : LEX g) (o1 : OP g) : 
       parse_tree g -> parse_tree g -> Prop :=
   | Atomic_LInsert_One l2 :
       linsert_one pr l1 o1 (AtomicNode l2)
         (InfixNode (AtomicNode l1) o1 (AtomicNode l2))
   | Infix_LInsert_One_1 t1 o2 t2 :
-      ~ conflict_pattern pr (CR_infix_infix o1 o2) ->
+      ~ i_conflict_pattern pr (CR_infix_infix o1 o2) ->
       linsert_one pr l1 o1 (InfixNode t1 o2 t2)
         (InfixNode (AtomicNode l1) o1 (InfixNode t1 o2 t2))
   | Infix_LInsert_One_2 t1 o2 t2 t1' :
-      conflict_pattern pr (CR_infix_infix o1 o2) ->
+      i_conflict_pattern pr (CR_infix_infix o1 o2) ->
       linsert_one pr l1 o1 t1 t1' ->
       linsert_one pr l1 o1 (InfixNode t1 o2 t2)
         (InfixNode t1' o2 t2)
@@ -258,190 +220,23 @@ Inductive linsert_one {g} (pr : drules g) (l1 : LEX g) (o1 : OP g) :
       linsert_one pr l1 o1 (PrefixNode o2 t)
         (InfixNode (AtomicNode l1) o1 (PrefixNode o2 t)).
 
-Lemma linsert_one_match {g} (pr : drules g) l o1 t t' :
-  linsert_one pr l o1 t t' ->
-  matches t' (InfixPatt HPatt o1 HPatt) \/
-  (exists o2, matches t (InfixPatt HPatt o2 HPatt) /\ matches t' (InfixPatt HPatt o2 HPatt)).
-Proof.
-  intros. inv H.
-  - left. apply InfixMatch; apply HMatch.
-  - left. apply InfixMatch; apply HMatch.
-  - right. exists o2. split; apply InfixMatch; apply HMatch.
-  - left. apply InfixMatch; apply HMatch.
-Qed.
-
-Lemma conflict_pattern_cases {O} (pr : drules O) (q : tree_pattern O) (P : Prop) :
-  (forall o1 o2, q = CL_infix_infix o1 o2 -> P) ->
-  (forall o1 o2, q = CR_infix_infix o1 o2 -> P) ->
-  (forall o1 o2, q = CL_infix_prefix o1 o2 -> P) ->
-  (forall o1 o2, q = CR_prefix_infix o1 o2 -> P) ->
-  (conflict_pattern pr q -> P).
-Proof.
-  intros. inv H3; eauto.
-Qed.
-
-Lemma linsert_one_safe {g} (pr : drules g) l1 o1 t t' :
-  safe_pr pr ->
-  conflict_free (conflict_pattern pr) t ->
-  linsert_one pr l1 o1 t t' ->
-  conflict_free (conflict_pattern pr) t'.
-Proof.
-  intro H_safe. intros. induction H0.
-  - apply Infix_cf; auto using Atomic_cf.
-    intro. inv H0. inv H1. inv H0; inv H2.
-    inv H9. inv H4. inv H4. inv H9. inv H4.
-  - apply Infix_cf; auto using Atomic_cf.
-    intro. destruct H0. destruct H1 as [q]. inv H0.
-    inv H2. inv H1. inv H7; inv H6; inv H1.
-    auto using CLeft. auto using CPrio_infix_infix_2.
-  - inv H. apply Infix_cf; auto. clear H6 H7.
-    intro. destruct H as [q]. inv H.
-    eapply conflict_pattern_cases; try eassumption; intros; subst; inv H3.
-    + apply linsert_one_match in H1. destruct H1.
-      * inv H. inv H6. eauto using safe_infix_infix.
-      * destruct H5.
-        inv H. inv H1. inv H. inv H3. inv H6.
-        exists (CL_infix_infix o0 o3). split; auto.
-        unfold CL_infix_infix. auto using HMatch, InfixMatch.
-    + inv H11. destruct H5.
-      exists (CR_infix_infix o0 o3). split; auto.
-      unfold CR_infix_infix. auto using HMatch, InfixMatch.
-    + inv H6. inv H1.
-  - apply Infix_cf; auto using Atomic_cf.
-    intro. destruct H0 as [q]. inv H0.
-    inv H2. inv H1. inv H7; inv H6; inv H1.
-Qed.
-
-Lemma linsert_one_yield {g} (pr : drules g) l1 o1 t t' :
-  linsert_one pr l1 o1 t t' ->
-  yield t' = inl l1 :: inr o1 :: yield t.
-Proof.
-  intros. induction H; simpl; auto.
-  rewrite IHlinsert_one. reflexivity.
-Qed.
-
-Lemma linsert_one_wf {g} (pr : drules g) l o t t' :
-  wf_parse_tree g t ->
-  g.(prods) (InfixProd o) ->
-  linsert_one pr l o t t' ->
-  wf_parse_tree g t'.
-Proof.
-  intros. induction H1.
-  - auto using Infix_wf, Atomic_wf.
-  - auto using Infix_wf, Atomic_wf.
-  - inv H. auto using Infix_wf.
-  - auto using Infix_wf, Atomic_wf, Prefix_wf.
-Qed.
-
-Lemma linsert_one_exists {g} (pr : drules g) `{drules_dec pr} l o t :
-  exists t', linsert_one pr l o t t'.
-Proof.
-  induction t.
-  - eauto using Atomic_LInsert_One.
-  - assert (Decision (conflict_pattern pr (CR_infix_infix o o0))). {
-      auto using dec_conflict_pattern.
-    }
-    destruct IHt1, IHt2.
-    destruct H.
-    + eauto using Infix_LInsert_One_2.
-    + eauto using Infix_LInsert_One_1.
-  - eauto using Prefix_LInsert_One.
-Qed.
-
 Inductive linsert_op {g} (pr : drules g) o1 :
       parse_tree g -> parse_tree g -> Prop :=
   | Atomic_LInsert_Op l :
       linsert_op pr o1 (AtomicNode l)
         (PrefixNode o1 (AtomicNode l))
   | Infix_LInsert_Op_1 t1 o2 t2 :
-      ~ conflict_pattern pr (CR_prefix_infix o1 o2) ->
+      ~ i_conflict_pattern pr (CR_prefix_infix o1 o2) ->
       linsert_op pr o1 (InfixNode t1 o2 t2)
         (PrefixNode o1 (InfixNode t1 o2 t2))
   | Infix_LInsert_Op_2 t1 o2 t2 t1' :
-      conflict_pattern pr (CR_prefix_infix o1 o2) ->
+      i_conflict_pattern pr (CR_prefix_infix o1 o2) ->
       linsert_op pr o1 t1 t1' ->
       linsert_op pr o1 (InfixNode t1 o2 t2)
         (InfixNode t1' o2 t2)
   | Prefix_LInsert_Op o2 t :
       linsert_op pr o1 (PrefixNode o2 t)
         (PrefixNode o1 (PrefixNode o2 t)).
-
-Lemma linsert_op_match {g} (pr : drules g) o1 t t' :
-  linsert_op pr o1 t t' ->
-  matches t' (PrefixPatt o1 HPatt) \/
-  (exists o2, matches t (InfixPatt HPatt o2 HPatt) /\ matches t' (InfixPatt HPatt o2 HPatt)).
-Proof.
-  intros. inv H; auto using PrefixMatch, HMatch.
-  right. exists o2. auto using InfixMatch, HMatch.
-Qed. 
-
-Lemma linsert_op_safe {g} (pr : drules g) o1 t t' :
-  safe_pr pr ->
-  conflict_free (conflict_pattern pr) t ->
-  linsert_op pr o1 t t' ->
-  conflict_free (conflict_pattern pr) t'.
-Proof.
-  intro H_safe. intros. induction H0.
-  - apply Prefix_cf; auto using Atomic_cf.
-    intro. inv H0. inv H1. inv H0; inv H2.
-    inv H3.
-  - apply Prefix_cf; auto.
-    intro. destruct H0.
-    destruct H1 as [q]. inv H0. inv H1; inv H2.
-    inv H3. auto using CPrio_prefix_infix.
-  - inv H. apply Infix_cf; auto.
-    intro. destruct H5. destruct H as [q]. inv H.
-    eapply conflict_pattern_cases; try eassumption; intros; subst; inv H3.
-    + apply linsert_op_match in H1. destruct H1.
-      * inv H. inv H5.
-      * inv H. inv H1. inv H. inv H5. inv H3.
-        eexists. split. eassumption.
-        unfold CL_infix_infix. auto using InfixMatch, HMatch.
-    + inv H12.
-      eexists. split. eassumption.
-      unfold CR_infix_infix. auto using InfixMatch, HMatch.
-    + apply linsert_op_match in H1. destruct H1.
-      * exfalso. inv H5. inv H. eauto using safe_infix_prefix.
-      * inv H. inv H1. inv H5. inv H3.
-  - apply Prefix_cf; auto.
-    intro. inv H0. inv H1. inv H0; inv H2. inv H3.
-Qed.
-
-Lemma linsert_op_yield {g} (pr : drules g) o1 t t' :
-  linsert_op pr o1 t t' ->
-  yield t' = inr o1 :: yield t.
-Proof.
-  intros. induction H; simpl; auto.
-  rewrite IHlinsert_op. reflexivity.
-Qed.
-
-Lemma linsert_op_wf {g} (pr : drules g) o1 t t' :
-  wf_parse_tree g t ->
-  g.(prods) (PrefixProd o1) ->
-  linsert_op pr o1 t t' ->
-  wf_parse_tree g t'.
-Proof.
-  intros. induction H1.
-  - auto using Prefix_wf, Atomic_wf.
-  - auto using Prefix_wf, Infix_wf.
-  - inv H. auto using Infix_wf.
-  - auto using Prefix_wf.
-Qed.
-
-Lemma linsert_op_exists {g} (pr : drules g) `{drules_dec pr} o t :
-  exists t', linsert_op pr o t t'.
-Proof.
-  induction t.
-  - eauto using Atomic_LInsert_Op.
-  - assert (Decision (conflict_pattern pr (CR_prefix_infix o o0))). {
-      auto using dec_conflict_pattern.
-    }
-    destruct IHt1, IHt2.
-    destruct H.
-    + eauto using Infix_LInsert_Op_2.
-    + eauto using Infix_LInsert_Op_1.
-  - eauto using Prefix_LInsert_Op.
-Qed.
 
 Inductive linsert {g} (pr : drules g) :
       parse_tree g -> OP g -> parse_tree g -> parse_tree g -> Prop :=
@@ -457,59 +252,6 @@ Inductive linsert {g} (pr : drules g) :
       linsert_op pr o1 t' t'' ->
       linsert pr (PrefixNode o1 t1) o2 t t''.
 
-Lemma linsert_yield {g} (pr : drules g) o t1 t2 t' :
-  linsert pr t1 o t2 t' ->
-  yield t' = yield t1 ++ inr o :: yield t2.
-Proof.
-  intro. induction H; simpl; eauto using linsert_one_yield.
-  - rewrite IHlinsert2. rewrite IHlinsert1.
-    simplify_list_eq. reflexivity.
-  - apply linsert_op_yield in H0.
-    rewrite H0. rewrite IHlinsert.
-    reflexivity.
-Qed.
-
-Lemma linsert_safe {g} (pr : drules g) o t1 t2 t' :
-  safe_pr pr ->
-  conflict_free (conflict_pattern pr) t2 ->
-  linsert pr t1 o t2 t' ->
-  conflict_free (conflict_pattern pr) t'.
-Proof.
-  intros. induction H1; eauto using linsert_one_safe, linsert_op_safe.
-Qed.
-
-Lemma linsert_wf {g} (pr : drules g) o t1 t2 t' :
-  wf_parse_tree g t1 ->
-  g.(prods) (InfixProd o) ->
-  wf_parse_tree g t2 ->
-  linsert pr t1 o t2 t' ->
-  wf_parse_tree g t'.
-Proof.
-  intros. induction H2.
-  - eauto using linsert_one_wf.
-  - inv H. auto.
-  - inv H. eauto using linsert_op_wf.
-Qed.
-
-Lemma linsert_exists {g} (pr : drules g) `{drules_dec pr} o t1 t2 :
-  exists t', linsert pr t1 o t2 t'.
-Proof.
-  revert o t2. induction t1; intros.
-  - assert (exists t', linsert_one pr l o t2 t'). {
-      auto using linsert_one_exists.
-    }
-    destruct H. eauto using Atomic_LInsert.
-  - specialize IHt1_2 with o0 t2. destruct IHt1_2.
-    specialize IHt1_1 with o x. destruct IHt1_1.
-    eauto using Infix_LInsert.
-  - specialize IHt1 with o0 t2. destruct IHt1.
-    assert (exists t', linsert_op pr o x t'). {
-      auto using linsert_op_exists.
-    }
-    destruct H0.
-    eauto using Prefix_LInsert.
-Qed.
-
 Inductive fix_tree {g} (pr : drules g) : parse_tree g -> parse_tree g -> Prop :=
   | Atomic_fix l :
       fix_tree pr (AtomicNode l) (AtomicNode l)
@@ -522,74 +264,4 @@ Inductive fix_tree {g} (pr : drules g) : parse_tree g -> parse_tree g -> Prop :=
       linsert_op pr o t1' t' ->
       fix_tree pr (PrefixNode o t1) t'.
 
-Lemma fix_tree_safe {g} (pr : drules g) t t' :
-  safe_pr pr ->
-  fix_tree pr t t' ->
-  conflict_free (conflict_pattern pr) t'.
-Proof.
-  intros. induction H0.
-  - apply Atomic_cf.
-  - eauto using linsert_safe.
-  - eauto using linsert_op_safe.
-Qed.
-
-Lemma fix_tree_yield {g} (pr : drules g) t t' :
-  fix_tree pr t t' ->
-  yield t' = yield t.
-Proof.
-  intros. induction H; simpl.
-  - reflexivity.
-  - apply linsert_yield in H0. rewrite H0.
-    rewrite IHfix_tree.
-    reflexivity.
-  - apply linsert_op_yield in H0. rewrite H0.
-    rewrite IHfix_tree.
-    reflexivity.
-Qed.
-
-Lemma fix_tree_wf {g} (pr : drules g) t t' :
-  wf_parse_tree g t ->
-  fix_tree pr t t' ->
-  wf_parse_tree g t'.
-Proof.
-  intros. induction H0.
-  - apply Atomic_wf.
-  - inv H. eauto using linsert_wf.
-  - inv H. eauto using linsert_op_wf.
-Qed.
-
-Lemma fix_tree_exists {g} (pr : drules g) `{drules_dec pr} t :
-  exists t', fix_tree pr t t'.
-Proof.
-  induction t.
-  - eauto using Atomic_fix.
-  - destruct IHt2.
-    assert (exists t', linsert pr t1 o x t'). {
-      auto using linsert_exists.
-    }
-    destruct H0.
-    eauto using Infix_fix.
-  - destruct IHt.
-    assert (exists t', linsert_op pr o x t'). {
-      auto using linsert_op_exists.
-    }
-    destruct H0.
-    eauto using Prefix_fix.
-Qed.
-
-Theorem safety {g} (pr : drules g) `{drules_dec pr} w :
-  safe_pr pr ->
-  language w -> dlanguage pr w.
-Proof.
-  unfold language, dlanguage. intros.
-  destruct H0 as [t]. inv H0.
-  assert (exists t', fix_tree pr t t'). {
-    auto using fix_tree_exists.
-  }
-  destruct H0 as [t'].
-  exists t'.
-  split; try split.
-  - eauto using fix_tree_wf.
-  - eauto using fix_tree_yield.
-  - eauto using fix_tree_safe.
-Qed.
+End IPPGrammar.
