IPPGrammarTheorems.v
@@ -1,0 +1,495 @@
+Require Import MyUtils.
+Load IPPGrammar.
+
+Section IPPGrammarTheorems.
+
+Arguments InfixProd {_} _.
+Arguments PrefixProd {_} _.
+
+Arguments HPatt {_}.
+Arguments InfixPatt {_} _ _ _.
+Arguments PrefixPatt {_} _ _.
+
+Arguments prio {_} _ _ _.
+Arguments left_a {_} _ _ _.
+Arguments right_a {_} _ _ _.
+
+(* Existential Lemmas *)
+
+Lemma dec_i_conflict_pattern {g} (pr : drules g) `{drules_dec pr} (q : tree_pattern g) :
+  Decision (i_conflict_pattern pr q).
+Proof.
+  destruct drules_dec0.
+  unfold Decision. destruct q.
+  - right. intro. inv H.
+  - destruct q1, q2.
+    + right. intro. inv H.
+    + destruct q2_1. destruct q2_2.
+      * replace (InfixPatt HPatt o (InfixPatt HPatt o0 HPatt)) with (CR_infix_infix o o0); try reflexivity.
+        specialize dec_prio0 with (p1 := InfixProd o) (p2 := InfixProd o0).
+        specialize dec_left_a0 with (p1 := InfixProd o) (p2 := InfixProd o0).
+        destruct dec_prio0, dec_left_a0; auto using CPrio_infix_infix_2, CLeft.
+        right. intro. inv H; contradiction.
+      * right. intro. inv H.
+      * right. intro. inv H.
+      * right. intro. inv H.
+      * right. intro. inv H.
+    + right. intro. inv H.
+    + destruct q1_1. destruct q1_2.
+      * replace (InfixPatt (InfixPatt HPatt o0 HPatt) o HPatt) with (CL_infix_infix o o0); try reflexivity.
+        specialize dec_prio0 with (p1 := InfixProd o) (p2 := InfixProd o0).
+        specialize dec_right_a0 with (p1 := InfixProd o) (p2 := InfixProd o0).
+        destruct dec_prio0, dec_right_a0; auto using CPrio_infix_infix_1, CRight.
+        right. intro. inv H; contradiction.
+      * right. intro. inv H.
+      * right. intro. inv H.
+      * right. intro. inv H.
+      * right. intro. inv H.
+    + right. intro. inv H.
+    + right. intro. inv H.
+    + right. intro. inv H.
+    + right. intro. inv H.
+    + right. intro. inv H.
+  - destruct q.
+    + right. intro. inv H.
+    + destruct q1, q2.
+      * replace (PrefixPatt o (InfixPatt HPatt o0 HPatt)) with (CR_prefix_infix o o0); try reflexivity.
+        specialize dec_prio0 with (p1 := PrefixProd o) (p2 := InfixProd o0).
+        destruct dec_prio0; auto using CPrio_prefix_infix.
+        right. intro. inv H. contradiction.
+      * right. intro. inv H.
+      * right. intro. inv H.
+      * right. intro. inv H.
+      * right. intro. inv H.
+      * right. intro. inv H.
+      * right. intro. inv H.
+      * right. intro. inv H.
+      * right. intro. inv H.
+    + right. intro. inv H.
+Qed.
+
+Lemma linsert_one_exists {g} (pr : drules g) `{drules_dec pr} l o t :
+  exists t', linsert_one pr l o t t'.
+Proof.
+  induction t.
+  - eauto using Atomic_LInsert_One.
+  - assert (Decision (i_conflict_pattern pr (CR_infix_infix o o0))). {
+      auto using dec_i_conflict_pattern.
+    }
+    destruct IHt1, IHt2.
+    destruct H.
+    + eauto using Infix_LInsert_One_2.
+    + eauto using Infix_LInsert_One_1.
+  - eauto using Prefix_LInsert_One.
+Qed.
+
+Lemma linsert_op_exists {g} (pr : drules g) `{drules_dec pr} o t :
+  exists t', linsert_op pr o t t'.
+Proof.
+  induction t.
+  - eauto using Atomic_LInsert_Op.
+  - assert (Decision (i_conflict_pattern pr (CR_prefix_infix o o0))). {
+      auto using dec_i_conflict_pattern.
+    }
+    destruct IHt1, IHt2.
+    destruct H.
+    + eauto using Infix_LInsert_Op_2.
+    + eauto using Infix_LInsert_Op_1.
+  - eauto using Prefix_LInsert_Op.
+Qed.
+
+Lemma linsert_exists {g} (pr : drules g) `{drules_dec pr} o t1 t2 :
+  exists t', linsert pr t1 o t2 t'.
+Proof.
+  revert o t2. induction t1; intros.
+  - assert (exists t', linsert_one pr l o t2 t'). {
+      auto using linsert_one_exists.
+    }
+    destruct H. eauto using Atomic_LInsert.
+  - specialize IHt1_2 with o0 t2. destruct IHt1_2.
+    specialize IHt1_1 with o x. destruct IHt1_1.
+    eauto using Infix_LInsert.
+  - specialize IHt1 with o0 t2. destruct IHt1.
+    assert (exists t', linsert_op pr o x t'). {
+      auto using linsert_op_exists.
+    }
+    destruct H0.
+    eauto using Prefix_LInsert.
+Qed.
+
+Lemma fix_tree_exists {g} (pr : drules g) `{drules_dec pr} t :
+  exists t', fix_tree pr t t'.
+Proof.
+  induction t.
+  - eauto using Atomic_fix.
+  - destruct IHt2.
+    assert (exists t', linsert pr t1 o x t'). {
+      auto using linsert_exists.
+    }
+    destruct H0.
+    eauto using Infix_fix.
+  - destruct IHt.
+    assert (exists t', linsert_op pr o x t'). {
+      auto using linsert_op_exists.
+    }
+    destruct H0.
+    eauto using Prefix_fix.
+Qed.
+
+(* Well-formedness Lemmas *)
+
+Lemma linsert_one_wf {g} (pr : drules g) l o t t' :
+  wf_parse_tree g t ->
+  g.(prods) (InfixProd o) ->
+  linsert_one pr l o t t' ->
+  wf_parse_tree g t'.
+Proof.
+  intros. induction H1.
+  - auto using Infix_wf, Atomic_wf.
+  - auto using Infix_wf, Atomic_wf.
+  - inv H. auto using Infix_wf.
+  - auto using Infix_wf, Atomic_wf, Prefix_wf.
+Qed.
+
+Lemma linsert_op_wf {g} (pr : drules g) o1 t t' :
+  wf_parse_tree g t ->
+  g.(prods) (PrefixProd o1) ->
+  linsert_op pr o1 t t' ->
+  wf_parse_tree g t'.
+Proof.
+  intros. induction H1.
+  - auto using Prefix_wf, Atomic_wf.
+  - auto using Prefix_wf, Infix_wf.
+  - inv H. auto using Infix_wf.
+  - auto using Prefix_wf.
+Qed.
+
+Lemma linsert_wf {g} (pr : drules g) o t1 t2 t' :
+  wf_parse_tree g t1 ->
+  g.(prods) (InfixProd o) ->
+  wf_parse_tree g t2 ->
+  linsert pr t1 o t2 t' ->
+  wf_parse_tree g t'.
+Proof.
+  intros. induction H2.
+  - eauto using linsert_one_wf.
+  - inv H. auto.
+  - inv H. eauto using linsert_op_wf.
+Qed.
+
+Lemma fix_tree_wf {g} (pr : drules g) t t' :
+  wf_parse_tree g t ->
+  fix_tree pr t t' ->
+  wf_parse_tree g t'.
+Proof.
+  intros. induction H0.
+  - apply Atomic_wf.
+  - inv H. eauto using linsert_wf.
+  - inv H. eauto using linsert_op_wf.
+Qed.
+
+(* Yield Lemmas *)
+
+Lemma linsert_one_yield {g} (pr : drules g) l1 o1 t t' :
+  linsert_one pr l1 o1 t t' ->
+  yield t' = inl l1 :: inr o1 :: yield t.
+Proof.
+  intros. induction H; simpl; auto.
+  rewrite IHlinsert_one. reflexivity.
+Qed.
+
+Lemma linsert_op_yield {g} (pr : drules g) o1 t t' :
+  linsert_op pr o1 t t' ->
+  yield t' = inr o1 :: yield t.
+Proof.
+  intros. induction H; simpl; auto.
+  rewrite IHlinsert_op. reflexivity.
+Qed.
+
+Lemma linsert_yield {g} (pr : drules g) o t1 t2 t' :
+  linsert pr t1 o t2 t' ->
+  yield t' = yield t1 ++ inr o :: yield t2.
+Proof.
+  intro. induction H; simpl; eauto using linsert_one_yield.
+  - rewrite IHlinsert2. rewrite IHlinsert1.
+    simplify_list_eq. reflexivity.
+  - apply linsert_op_yield in H0.
+    rewrite H0. rewrite IHlinsert.
+    reflexivity.
+Qed.
+
+Lemma fix_tree_yield {g} (pr : drules g) t t' :
+  fix_tree pr t t' ->
+  yield t' = yield t.
+Proof.
+  intros. induction H; simpl.
+  - reflexivity.
+  - apply linsert_yield in H0. rewrite H0.
+    rewrite IHfix_tree.
+    reflexivity.
+  - apply linsert_op_yield in H0. rewrite H0.
+    rewrite IHfix_tree.
+    reflexivity.
+Qed.
+
+(* pr safety lemmas *)
+
+Lemma safe_infix_infix {g} (pr : drules g) o1 o2 :
+  safe_pr pr ->
+  i_conflict_pattern pr (CL_infix_infix o1 o2) ->
+  i_conflict_pattern pr (CR_infix_infix o2 o1) ->
+  False.
+Proof.
+  intros H_safe H_CL H_CR. unfold safe_pr in H_safe.
+  inv H_CL; inv H_CR; eauto.
+Qed.
+
+Lemma safe_infix_prefix {g} (pr : drules g) o1 o2 :
+  safe_pr pr ->
+  rm_conflict_pattern pr (CL_infix_prefix o1 o2) ->
+  i_conflict_pattern pr (CR_prefix_infix o2 o1) ->
+  False.
+Proof.
+  intros. unfold safe_pr in H.
+  inv H0; inv H1; eauto.
+Qed.
+
+(* general insertion lemmas *)
+
+Lemma linsert_one_match {g} (pr : drules g) l o1 t t' :
+  linsert_one pr l o1 t t' ->
+  matches t' (InfixPatt HPatt o1 HPatt) \/
+  (exists o2, matches t (InfixPatt HPatt o2 HPatt) /\ matches t' (InfixPatt HPatt o2 HPatt)).
+Proof.
+  intros. inv H.
+  - left. apply InfixMatch; apply HMatch.
+  - left. apply InfixMatch; apply HMatch.
+  - right. exists o2. split; apply InfixMatch; apply HMatch.
+  - left. apply InfixMatch; apply HMatch.
+Qed.
+
+Lemma linsert_op_match {g} (pr : drules g) o1 t t' :
+  linsert_op pr o1 t t' ->
+  matches t' (PrefixPatt o1 HPatt) \/
+  (exists o2, matches t (InfixPatt HPatt o2 HPatt) /\ matches t' (InfixPatt HPatt o2 HPatt)).
+Proof.
+  intros. inv H; auto using PrefixMatch, HMatch.
+  right. exists o2. auto using InfixMatch, HMatch.
+Qed. 
+
+(* i-conflict-free lemmas *)
+
+Lemma i_conflict_pattern_cases {O} (pr : drules O) (q : tree_pattern O) (P : Prop) :
+  (forall o1 o2, q = CL_infix_infix o1 o2 -> P) ->
+  (forall o1 o2, q = CR_infix_infix o1 o2 -> P) ->
+  (forall o1 o2, q = CR_prefix_infix o1 o2 -> P) ->
+  (i_conflict_pattern pr q -> P).
+Proof.
+  intros. inv H2; eauto.
+Qed.
+
+Lemma linsert_one_icfree {g} (pr : drules g) l1 o1 t t' :
+  safe_pr pr ->
+  i_conflict_free (i_conflict_pattern pr) t ->
+  linsert_one pr l1 o1 t t' ->
+  i_conflict_free (i_conflict_pattern pr) t'.
+Proof.
+  intro H_safe. intros. induction H0.
+  - apply Infix_cf; auto using Atomic_cf.
+    intro. inv H0. inv H1. inv H0; inv H2.
+    inv H9. inv H4. inv H4. inv H9.
+  - apply Infix_cf; auto using Atomic_cf.
+    intro. destruct H0. destruct H1 as [q]. inv H0.
+    inv H2. inv H1. inv H7; inv H6; inv H1.
+    auto using CLeft. auto using CPrio_infix_infix_2.
+  - inv H. apply Infix_cf; auto. clear H6 H7.
+    intro. destruct H as [q]. inv H.
+    eapply i_conflict_pattern_cases; try eassumption; intros; subst; inv H3.
+    + apply linsert_one_match in H1. destruct H1.
+      * inv H. inv H6. eauto using safe_infix_infix.
+      * destruct H5.
+        inv H. inv H1. inv H. inv H3. inv H6.
+        exists (CL_infix_infix o0 o3). split; auto.
+        unfold CL_infix_infix. auto using HMatch, InfixMatch.
+    + inv H11. destruct H5.
+      exists (CR_infix_infix o0 o3). split; auto.
+      unfold CR_infix_infix. auto using HMatch, InfixMatch.
+  - apply Infix_cf; auto using Atomic_cf.
+    intro. destruct H0 as [q]. inv H0.
+    inv H2. inv H1. inv H7; inv H6; inv H1.
+Qed.
+
+Lemma linsert_op_icfree {g} (pr : drules g) o1 t t' :
+  safe_pr pr ->
+  i_conflict_free (i_conflict_pattern pr) t ->
+  linsert_op pr o1 t t' ->
+  i_conflict_free (i_conflict_pattern pr) t'.
+Proof.
+  intro H_safe. intros. induction H0.
+  - apply Prefix_cf; auto using Atomic_cf.
+    intro. inv H0. inv H1. inv H0; inv H2.
+    inv H3.
+  - apply Prefix_cf; auto.
+    intro. destruct H0.
+    destruct H1 as [q]. inv H0. inv H1; inv H2.
+    inv H3. auto using CPrio_prefix_infix.
+  - inv H. apply Infix_cf; auto.
+    intro. destruct H5. destruct H as [q]. inv H.
+    eapply i_conflict_pattern_cases; try eassumption; intros; subst; inv H3.
+    + apply linsert_op_match in H1. destruct H1.
+      * inv H. inv H5.
+      * inv H. inv H1. inv H. inv H5. inv H3.
+        eexists. split. eassumption.
+        unfold CL_infix_infix. auto using InfixMatch, HMatch.
+    + inv H12.
+      eexists. split. eassumption.
+      unfold CR_infix_infix. auto using InfixMatch, HMatch.
+  - apply Prefix_cf; auto.
+    intro. inv H0. inv H1. inv H0; inv H2. inv H3.
+Qed.
+
+Lemma linsert_icfree {g} (pr : drules g) o t1 t2 t' :
+  safe_pr pr ->
+  i_conflict_free (i_conflict_pattern pr) t2 ->
+  linsert pr t1 o t2 t' ->
+  i_conflict_free (i_conflict_pattern pr) t'.
+Proof.
+  intros. induction H1; eauto using linsert_one_icfree, linsert_op_icfree.
+Qed.
+
+Lemma fix_tree_icfree {g} (pr : drules g) t t' :
+  safe_pr pr ->
+  fix_tree pr t t' ->
+  i_conflict_free (i_conflict_pattern pr) t'.
+Proof.
+  intros. induction H0.
+  - apply Atomic_cf.
+  - eauto using linsert_icfree.
+  - eauto using linsert_op_icfree.
+Qed.
+
+(* rm-conflict-free lemmas *)
+
+Lemma matches_rm_hpatt {g} (t : parse_tree g) :
+  matches_rm t HPatt.
+Proof.
+  apply Match_rm. apply HMatch.
+Qed.
+
+Lemma linsert_one_matches_rm {g} (pr : drules g) l1 o1 t o t' :
+  linsert_one pr l1 o1 t t' ->
+  matches_rm t' (PrefixPatt o HPatt) ->
+  matches_rm t (PrefixPatt o HPatt).
+Proof.
+  intros. inv H.
+  - inv H0. inv H. inv H4. inv H.
+  - inv H0. inv H. assumption.
+  - inv H0. inv H. auto using InfixMatch_rm.
+  - inv H0. inv H. assumption.
+Qed.
+
+Lemma linsert_one_drmcfree {g} (pr : drules g) l1 o1 t t' :
+  safe_pr pr ->
+  drm_conflict_free (rm_conflict_pattern pr) t ->
+  linsert_one pr l1 o1 t t' ->
+  drm_conflict_free (rm_conflict_pattern pr) t'.
+Proof.
+  intros. induction H1.
+  - apply Infix_drmcf; auto using Atomic_drmcf.
+    intro. destruct H1 as [q].
+    inv H1. inv H2. inv H3. inv H5. inv H2.
+  - apply Infix_drmcf; auto using Atomic_drmcf.
+    intro. destruct H2 as [q].
+    inv H2. inv H3. inv H4. inv H6. inv H3.
+  - inv H0. apply Infix_drmcf; auto.
+    intro. destruct H0 as [q]. inv H0.
+    destruct H6. exists q. split. assumption.
+    inv H3. inv H4.
+    apply InfixMatch_drm; eauto using matches_rm_hpatt, linsert_one_matches_rm.
+  - apply Infix_drmcf; auto using Atomic_drmcf.
+    intro. destruct H1 as [q]. inv H1.
+    inv H2. inv H3. inv H5. inv H2.
+Qed.
+
+Lemma linsert_op_matches_rm {g} (pr : drules g) o1 t o t' :
+  linsert_op pr o1 t t' ->
+  matches_rm t' (PrefixPatt o HPatt) ->
+  matches_rm t (PrefixPatt o HPatt) \/ o = o1.
+Proof.
+  intros. inv H.
+  - inv H0.
+    + inv H. auto.
+    + inv H3. inv H.
+  - inv H0; auto.
+    inv H. auto.
+  - inv H0. inv H.
+    left. auto using InfixMatch_rm.
+  - inv H0; auto.
+    inv H. auto.
+Qed.
+
+Lemma linsert_op_drmcfree {g} (pr : drules g) o1 t t' :
+  safe_pr pr ->
+  drm_conflict_free (rm_conflict_pattern pr) t ->
+  linsert_op pr o1 t t' ->
+  drm_conflict_free (rm_conflict_pattern pr) t'.
+Proof.
+  intros. induction H1.
+  - apply Prefix_drmcf; auto using Atomic_drmcf.
+    intro. inv H1. inv H2. inv H3. inv H1.
+  - apply Prefix_drmcf; auto.
+    intro. inv H2. inv H3. inv H2. inv H4.
+  - inv H0. apply Infix_drmcf; auto.
+    intro. destruct H0 as [q]. inv H0. inv H3. inv H4.
+    eapply linsert_op_matches_rm in H2; eauto.
+    inv H2.
+    + destruct H6.
+      eexists. split. eauto using CPrio_infix_prefix.
+      unfold CL_infix_prefix. apply InfixMatch_drm; auto using Match_rm, HMatch.
+    + eapply safe_infix_prefix; eauto using CPrio_infix_prefix.
+  - apply Prefix_drmcf; auto.
+    intro. destruct H1 as [q]. inv H1.
+    inv H2. inv H3.
+Qed.
+
+Lemma linsert_drmcfree {g} (pr : drules g) t1 o t2 t' :
+  safe_pr pr ->
+  drm_conflict_free (rm_conflict_pattern pr) t2 ->
+  linsert pr t1 o t2 t' ->
+  drm_conflict_free (rm_conflict_pattern pr) t'.
+Proof.
+  intros. induction H1; eauto using linsert_one_drmcfree, linsert_op_drmcfree.
+Qed.
+
+Lemma fix_tree_drmcfree {g} (pr : drules g) t t' :
+  safe_pr pr ->
+  fix_tree pr t t' ->
+  drm_conflict_free (rm_conflict_pattern pr) t'.
+Proof.
+  intros. induction H0.
+  - apply Atomic_drmcf.
+  - eauto using linsert_drmcfree.
+  - eauto using linsert_op_drmcfree.
+Qed.
+
+(* safety *)
+
+Theorem safety {g} (pr : drules g) `{drules_dec pr} w :
+  safe_pr pr ->
+  language w -> dlanguage pr w.
+Proof.
+  unfold language, dlanguage. intros.
+  destruct H0 as [t]. inv H0.
+  assert (exists t', fix_tree pr t t'). {
+    auto using fix_tree_exists.
+  }
+  destruct H0 as [t'].
+  exists t'.
+  split; try split; try split.
+  - eauto using fix_tree_wf.
+  - eauto using fix_tree_yield.
+  - eauto using fix_tree_icfree.
+  - eauto using fix_tree_drmcfree.
+Qed.
+
+End IPPGrammarTheorems.
